Put back actions in definition of the effect

iodiv/TauIODiv.fst
@@ -68,6 +68,15 @@ let to_trace_append_pat t t' :
 let act_call (ac : io_sig.act) (x : io_sig.arg ac) : IODIV (io_sig.res x) (iodiv_act ac x) =
   IODIV?.reflect (iodiv_call ac x)
 
+let open_file (s : string) : IODiv file_descr (requires fun hist -> True) (ensures fun hist r -> terminates r /\ ret_trace r == [ EOpenfile s (result r) ]) =
+  act_call Openfile s
+
+let read (fd : file_descr) : IODiv string (requires fun hist -> is_open fd hist) (ensures fun hist r -> terminates r /\ ret_trace r == [ ERead fd (result r) ]) =
+  act_call Read fd
+
+let close (fd : file_descr) : IODiv unit (requires fun hist -> is_open fd hist) (ensures fun hist r -> terminates r /\ ret_trace r == [ EClose fd ]) =
+  act_call Close fd
+
 let iter #index #a #w (f : (j : index) -> IODIV (either index a) (w j)) (i : index) : IODIV a (i_iter w i) =
   IODIV?.reflect (dm_iter (fun j -> reify (f j)) i)
 
