iodiv/TestTauIODiv.fst
@@ -17,15 +17,14 @@ open DivFree
 open DivFreeTauSpec
 open DivFreeTauDM
 
-let open_file (s : string) : IODiv file_descr (requires fun hist -> True) (ensures fun hist r -> terminates r /\ ret_trace r == [ EOpenfile s (result r) ]) =
-  act_call Openfile s
+// let open_file (s : string) : IODiv file_descr (requires fun hist -> True) (ensures fun hist r -> terminates r /\ ret_trace r == [ EOpenfile s (result r) ]) =
+//   act_call Openfile s
 
-let read (fd : file_descr) : IODiv string (requires fun hist -> is_open fd hist) (ensures fun hist r -> terminates r /\ ret_trace r == [ ERead fd (result r) ]) =
-  act_call Read fd
+// let read (fd : file_descr) : IODiv string (requires fun hist -> is_open fd hist) (ensures fun hist r -> terminates r /\ ret_trace r == [ ERead fd (result r) ]) =
+//   act_call Read fd
 
-let close (fd : file_descr) : IODiv unit (requires fun hist -> is_open fd hist) (ensures fun hist r -> terminates r /\ ret_trace r == [ EClose fd ]) =
-  act_call Close fd
-
+// let close (fd : file_descr) : IODiv unit (requires fun hist -> is_open fd hist) (ensures fun hist r -> terminates r /\ ret_trace r == [ EClose fd ]) =
+//   act_call Close fd
 
 let open_file' = act_call Openfile
 let read' = act_call Read
